progs/conclib.v
@@ -3390,42 +3390,44 @@ Notation "'TYPE' A 'WITH'  x1 : t1 , x2 : t2 , x3 : t3 , x4 : t4 , x5 : t5 , x6 
 
 (* automation for dependent funspecs *)
 Definition call_setup2'
-  (cs: compspecs) Qtemp Qvar a Delta P Q R  
+  (cs: compspecs) Qtemp Qvar G a Delta P Q R  
    argsig retty cc ts (A: rmaps.TypeTree)  Pre Post NEPre NEPost
   (bl: list expr) (vl : list val)
   (Qactuals : PTree.t _)
   (witness: functors.MixVariantFunctor._functor (rmaps.dependent_type_functor_rec ts A) mpred)
   (Frame: list mpred)
   (Ppre: list Prop) (Qpre : list localdef) (Rpre: list mpred)
-  (Qpre_temp : PTree.t _) (Qpre_var: PTree.t vardesc) :=
- call_setup1 cs Qtemp Qvar a Delta P Q R argsig retty cc A Pre Post NEPre NEPost bl vl Qactuals /\
+  (Qpre_temp : PTree.t _) (Qpre_var: PTree.t vardesc) G' :=
+ call_setup1 cs Qtemp Qvar G a Delta P Q R argsig retty cc A Pre Post NEPre NEPost bl vl Qactuals /\
   Pre ts witness = PROPx Ppre (LOCALx Qpre (SEPx Rpre)) /\
-  local2ptree Qpre = (Qpre_temp, Qpre_var, nil, nil) /\
+  local2ptree Qpre = (Qpre_temp, Qpre_var, nil, map gvars G') /\
   ENTAIL Delta, PROPx P (LOCALx Q (SEPx R))
            |-- !! Forall (check_one_temp_spec Qactuals) (PTree.elements Qpre_temp) /\
   ENTAIL Delta, PROPx P (LOCALx Q (SEPx R))
            |-- !! Forall (check_one_var_spec Qvar) (PTree.elements Qpre_var) /\
+  Forall (fun x => In x G) G' /\
   fold_right_sepcon R |-- fold_right_sepcon Rpre * fold_right_sepcon Frame.
 
 Lemma call_setup2'_i:
- forall  (cs: compspecs) Qtemp Qvar a Delta P Q R  
+ forall  (cs: compspecs) Qtemp Qvar (G: list globals) a Delta P Q R  
    argsig retty cc ts (A: rmaps.TypeTree) Pre Post NEPre NEPost
   (bl: list expr) (vl : list val)
   (Qactuals : PTree.t _)
-  (SETUP1: call_setup1 cs Qtemp Qvar a Delta P Q R argsig retty cc A Pre Post NEPre NEPost bl vl Qactuals)
+  (SETUP1: call_setup1 cs Qtemp Qvar G a Delta P Q R argsig retty cc A Pre Post NEPre NEPost bl vl Qactuals)
   (witness': functors.MixVariantFunctor._functor (rmaps.dependent_type_functor_rec ts A) mpred)
   (Frame: list mpred)
   (Ppre: list Prop) (Qpre : list localdef) (Rpre: list mpred)
-  (Qpre_temp : PTree.t _) (Qpre_var: PTree.t vardesc),
+  (Qpre_temp : PTree.t _) (Qpre_var: PTree.t vardesc) G',
   Pre ts witness' = PROPx Ppre (LOCALx Qpre (SEPx Rpre)) ->
-  local2ptree Qpre = (Qpre_temp, Qpre_var, nil, nil) ->
+  local2ptree Qpre = (Qpre_temp, Qpre_var, nil, map gvars G') ->
   ENTAIL Delta, PROPx P (LOCALx Q (SEPx R))
            |-- !! Forall (check_one_temp_spec Qactuals) (PTree.elements Qpre_temp) ->
   ENTAIL Delta, PROPx P (LOCALx Q (SEPx R))
            |-- !! Forall (check_one_var_spec Qvar) (PTree.elements Qpre_var)  ->
   fold_right_sepcon R |-- fold_right_sepcon Rpre * fold_right_sepcon Frame ->
-  call_setup2' cs Qtemp Qvar a Delta P Q R argsig retty cc ts A Pre Post NEPre NEPost bl vl Qactuals
-      witness' Frame Ppre Qpre Rpre Qpre_temp Qpre_var.
+  Forall (fun x => In x G) G' ->
+  call_setup2' cs Qtemp Qvar G a Delta P Q R argsig retty cc ts A Pre Post NEPre NEPost bl vl Qactuals
+      witness' Frame Ppre Qpre Rpre Qpre_temp Qpre_var G'.
 Proof.
  intros. split. auto. repeat split; auto.
 Qed.
@@ -3463,27 +3465,28 @@ Funspec type: " TA'')
 Ltac prove_call_setup' ts witness :=
  prove_call_setup1;
  [ .. | 
- match goal with |- call_setup1 _ _ _ _ _ _ _ _ _ _ _ ?A _ _ _ _ _ _ _ -> _ =>
+ match goal with |- call_setup1 _ _ _ _ _ _ _ _ _ _ _ _ ?A _ _ _ _ _ _ _ -> _ =>
       check_witness_type' ts A witness
  end;
  let H := fresh in
  intro H;
  let Frame := fresh "Frame" in evar (Frame: list mpred);
- exploit (call_setup2'_i _ _ _ _ _ _ _ _ _ _ _ ts _ _ _ _ _ _ _ _ H witness Frame); clear H;
+ exploit (call_setup2'_i _ _ _ _ _ _ _ _ _ _ _ _ ts _ _ _ _ _ _ _ _ H witness Frame); clear H;
  simpl functors.MixVariantFunctor._functor;
  [ reflexivity
  | check_prove_local2ptree
  | Forall_pTree_from_elements
  | Forall_pTree_from_elements
+ | try apply trivial_Forall_inclusion; try apply trivial_Forall_inclusion0
  | unfold fold_right_sepcon at 1 2; cancel_for_forward_call
  | 
  ]].
 
 Lemma semax_call_aux55:
- forall (cs: compspecs) (Qtemp: PTree.t val) (Qvar: PTree.t vardesc) (a: expr)
+ forall (cs: compspecs) (Qtemp: PTree.t val) (Qvar: PTree.t vardesc) G (a: expr)
      Delta P Q R argsig retty cc ts A Pre Post NEPre NEPost 
-    witness Frame bl Ppre Qpre Rpre Qactuals Qpre_temp Qpre_var vl
- (PTREE : local2ptree Q = (Qtemp, Qvar, nil, nil))
+    witness Frame bl Ppre Qpre Rpre Qactuals Qpre_temp Qpre_var G' vl
+ (PTREE : local2ptree Q = (Qtemp, Qvar, nil, map gvars G))
  (TC0 : ENTAIL Delta, PROPx P (LOCALx Q (SEPx R)) |-- tc_expr Delta a)
  (TC1 : ENTAIL Delta, PROPx P (LOCALx Q (SEPx R))
              |-- tc_exprlist Delta (argtypes argsig) bl)
@@ -3491,12 +3494,13 @@ Lemma semax_call_aux55:
               (explicit_cast_exprlist (argtypes argsig) bl)) = Some vl)
  (PTREE'' : pTree_from_elements (combine (var_names argsig) vl) = Qactuals)
  (PRE1 : Pre ts witness = PROPx Ppre (LOCALx Qpre (SEPx Rpre)))
- (PTREE' : local2ptree Qpre = (Qpre_temp, Qpre_var, nil, nil)) 
+ (PTREE' : local2ptree Qpre = (Qpre_temp, Qpre_var, nil, map gvars G')) 
  (CHECKTEMP : ENTAIL Delta, PROPx P (LOCALx Q (SEPx R))
             |-- !! Forall (check_one_temp_spec Qactuals)
                      (PTree.elements Qpre_temp))
  (CHECKVAR : ENTAIL Delta, PROPx P (LOCALx Q (SEPx R))
            |-- !! Forall (check_one_var_spec Qvar) (PTree.elements Qpre_var))
+ (CHECKG: Forall (fun x => In x G) G')
  (FRAME : fold_right_sepcon R
            |-- fold_right_sepcon Rpre * fold_right_sepcon Frame)
  (PPRE : fold_right_and True Ppre),
@@ -3552,7 +3556,7 @@ eapply derives_trans;[ apply andp_derives; [apply derives_refl | apply andp_left
  eapply derives_trans; [ apply IHl | ]. normalize.
 apply derives_extract_PROP; intro LEN.
 subst Qactuals. 
-clear - PTREE LEN PTREE' MSUBST CHECKVAR FRAME PPRE CHECKTEMP.
+clear - PTREE LEN PTREE' MSUBST CHECKVAR FRAME PPRE CHECKTEMP CHECKG.
  progress (autorewrite with norm1 norm2); normalize.
  eapply derives_trans.
  apply andp_right. apply andp_right. apply CHECKVAR. apply CHECKTEMP. apply derives_refl.
@@ -3580,7 +3584,7 @@ intro rho; unfold SEPx.
 +
  apply (local2ptree_soundness P _ R) in PTREE.
  simpl app in PTREE.
- apply msubst_eval_exprlist_eq with (P:=P)(R:=R)(Q:=nil) in MSUBST.
+ apply msubst_eval_exprlist_eq with (P:=P)(R:=R)(Q:=map gvars G) in MSUBST.
  rewrite PTREE.
  intro rho.
  unfold local, lift1. unfold_lift. simpl.
@@ -3601,7 +3605,7 @@ apply andp_left2. apply andp_left1.
     simpl; intros; auto.
  inv LEN.
  forget (argtypes argsig) as tys.
- cut (local (fold_right `and `True (map locald_denote (LocalD Qtemp Qvar nil))) rho |--
+ cut (local (fold_right `and `True (map locald_denote (LocalD Qtemp Qvar (map gvars G)))) rho |--
             `(local (fold_right `and `True (map locald_denote Qpre)))
                (fun rho => (make_args (var_names argsig) (eval_exprlist tys bl rho) rho)) rho).
  intro. eapply derives_trans; [apply H  |].
@@ -3612,20 +3616,30 @@ apply andp_left2. apply andp_left1.
  apply prop_derives; intro. forget (var_names argsig) as fl.
  forget (eval_exprlist tys bl rho) as vl.
  eapply check_specs_lemma; try eassumption.
-Qed.
+ clear - H.
+ apply fold_right_and_LocalD_e in H.
+  destruct H as [? [? ?]]. auto.
+ clear - CHECKG H1.
+ admit.  (* easy *)
+ clear - CHECKG H.
+ apply fold_right_and_LocalD_e in H.
+  destruct H as [? [? ?]].
+  clear - H1 CHECKG.
+ admit. (* easy *)
+Admitted.
 
 Lemma semax_call_id00_wow:
  forall  
-  (cs: compspecs) Qtemp Qvar a Delta P Q R  
+  (cs: compspecs) Qtemp Qvar a G Delta P Q R  
    argsig retty cc ts (A: rmaps.TypeTree)  Pre Post NEPre NEPost
    (witness: functors.MixVariantFunctor._functor (rmaps.dependent_type_functor_rec ts A) mpred) 
    (Frame: list mpred)
    (bl: list expr)
    (Ppre: list Prop) (Qpre : list localdef) (Rpre: list mpred)
-   (Qactuals Qpre_temp : PTree.t _) (Qpre_var: PTree.t vardesc)
+   (Qactuals Qpre_temp : PTree.t _) (Qpre_var: PTree.t vardesc) G'
    (vl : list val)
-   (SETUP: call_setup2' cs Qtemp Qvar a Delta P Q R argsig retty cc ts A Pre Post NEPre NEPost bl vl Qactuals
-      witness Frame Ppre Qpre Rpre Qpre_temp Qpre_var)
+   (SETUP: call_setup2' cs Qtemp Qvar G a Delta P Q R argsig retty cc ts A Pre Post NEPre NEPost bl vl Qactuals
+      witness Frame Ppre Qpre Rpre Qpre_temp Qpre_var G')
   Espec 
              (Post2: environ -> mpred)
              (B: Type)
@@ -3642,7 +3656,7 @@ Lemma semax_call_id00_wow:
 Proof.
 intros.
 destruct SETUP as [[PTREE [SPEC [ATY [TC0 [TC1 [MSUBST PTREE'']]]]]] 
-                            [PRE1 [PTREE' [CHECKTEMP [CHECKVAR FRAME]]]]].
+                            [PRE1 [PTREE' [CHECKTEMP [CHECKVAR [CHECKG FRAME]]]]]].
 apply SPEC. clear SPEC.
 eapply semax_pre_post'; [ | |
    apply (@semax_call0 Espec cs Delta A Pre Post NEPre NEPost 
@@ -3669,16 +3683,16 @@ Qed.
 
 Lemma semax_call_id1_wow:
  forall  
-  (cs: compspecs) Qtemp Qvar a Delta P Q R  
+  (cs: compspecs) Qtemp Qvar G a Delta P Q R  
    argsig retty cc ts (A: rmaps.TypeTree)  Pre Post NEPre NEPost
    (witness: functors.MixVariantFunctor._functor (rmaps.dependent_type_functor_rec ts A) mpred) 
    (Frame: list mpred)
    (bl: list expr)
    (Ppre: list Prop) (Qpre : list localdef) (Rpre: list mpred)
-   (Qactuals Qpre_temp : PTree.t _) (Qpre_var: PTree.t vardesc)
+   (Qactuals Qpre_temp : PTree.t _) (Qpre_var: PTree.t vardesc) G'
    (vl : list val)
-   (SETUP: call_setup2' cs Qtemp Qvar a Delta P Q R argsig retty cc ts A Pre Post NEPre NEPost bl vl Qactuals
-      witness Frame Ppre Qpre Rpre Qpre_temp Qpre_var)
+   (SETUP: call_setup2' cs Qtemp Qvar G a Delta P Q R argsig retty cc ts A Pre Post NEPre NEPost bl vl Qactuals
+      witness Frame Ppre Qpre Rpre Qpre_temp Qpre_var G')
    ret (Post2: environ -> mpred)  (Qnew: list localdef)
     (B: Type) (Ppost: B -> list Prop) (F: B -> val) (Rpost: B -> list mpred) Espec
    (TYret: typeof_temp Delta ret = Some retty)
@@ -3696,7 +3710,7 @@ Lemma semax_call_id1_wow:
 Proof.
 intros. 
 destruct SETUP as [[PTREE [SPEC [ATY [TC0 [TC1 [MSUBST PTREE'']]]]]] 
-                            [PRE1 [PTREE' [CHECKTEMP [CHECKVAR FRAME]]]]].
+                            [PRE1 [PTREE' [CHECKTEMP [CHECKVAR [CHECKG FRAME]]]]]].
 apply SPEC. clear SPEC.
 eapply semax_pre_post'; [ | |
    apply (@semax_call1 Espec cs Delta A Pre Post NEPre NEPost 
@@ -3734,16 +3748,16 @@ eapply semax_call_aux55; eauto.
 Qed.
 
 Lemma semax_call_id1_x_wow:
- forall  (cs: compspecs) Qtemp Qvar a Delta P Q R  
+ forall  (cs: compspecs) Qtemp Qvar G a Delta P Q R  
    argsig retty' cc ts (A: rmaps.TypeTree)  Pre Post NEPre NEPost
    (witness: functors.MixVariantFunctor._functor (rmaps.dependent_type_functor_rec ts A) mpred) 
    (Frame: list mpred)
    (bl: list expr)
    (Ppre: list Prop) (Qpre : list localdef) (Rpre: list mpred)
-   (Qactuals Qpre_temp : PTree.t _) (Qpre_var: PTree.t vardesc)
+   (Qactuals Qpre_temp : PTree.t _) (Qpre_var: PTree.t vardesc) G'
    (vl : list val)
-   (SETUP: call_setup2' cs Qtemp Qvar a Delta P Q R argsig retty' cc ts A Pre Post NEPre NEPost bl vl Qactuals
-      witness Frame Ppre Qpre Rpre Qpre_temp Qpre_var)
+   (SETUP: call_setup2' cs Qtemp Qvar G a Delta P Q R argsig retty' cc ts A Pre Post NEPre NEPost bl vl Qactuals
+      witness Frame Ppre Qpre Rpre Qpre_temp Qpre_var G')
    retty  Espec ret ret'
              (Post2: environ -> mpred)
              (Qnew: list localdef)
@@ -3855,16 +3869,16 @@ eapply semax_call_id1_wow; try eassumption; auto.
 Qed.
 
 Lemma semax_call_id1_y_wow:
- forall  (cs: compspecs) Qtemp Qvar a Delta P Q R  
+ forall  (cs: compspecs) Qtemp Qvar G a Delta P Q R  
    argsig retty' cc ts (A: rmaps.TypeTree)  Pre Post NEPre NEPost
    (witness: functors.MixVariantFunctor._functor (rmaps.dependent_type_functor_rec ts A) mpred) 
    (Frame: list mpred)
    (bl: list expr)
    (Ppre: list Prop) (Qpre : list localdef) (Rpre: list mpred)
-   (Qactuals Qpre_temp : PTree.t _) (Qpre_var: PTree.t vardesc)
+   (Qactuals Qpre_temp : PTree.t _) (Qpre_var: PTree.t vardesc) G'
    (vl : list val)
-   (SETUP: call_setup2' cs Qtemp Qvar a Delta P Q R argsig retty' cc ts A Pre Post NEPre NEPost bl vl Qactuals
-      witness Frame Ppre Qpre Rpre Qpre_temp Qpre_var)
+   (SETUP: call_setup2' cs Qtemp Qvar G a Delta P Q R argsig retty' cc ts A Pre Post NEPre NEPost bl vl Qactuals
+      witness Frame Ppre Qpre Rpre Qpre_temp Qpre_var G')
     Espec ret ret' (retty: type) 
              (Post2: environ -> mpred)
              (Qnew: list localdef)
@@ -3967,16 +3981,16 @@ Qed.
 
 Lemma semax_call_id01_wow:
  forall  
-  (cs: compspecs) Qtemp Qvar a Delta P Q R  
+  (cs: compspecs) Qtemp Qvar G a Delta P Q R  
    argsig retty cc ts (A: rmaps.TypeTree)  Pre Post NEPre NEPost
    (witness: functors.MixVariantFunctor._functor (rmaps.dependent_type_functor_rec ts A) mpred) 
    (Frame: list mpred)
    (bl: list expr)
    (Ppre: list Prop) (Qpre : list localdef) (Rpre: list mpred)
-   (Qactuals Qpre_temp : PTree.t _) (Qpre_var: PTree.t vardesc)
+   (Qactuals Qpre_temp : PTree.t _) (Qpre_var: PTree.t vardesc) G'
    (vl : list val)
-   (SETUP: call_setup2' cs Qtemp Qvar a Delta P Q R argsig retty cc ts A Pre Post NEPre NEPost bl vl Qactuals
-      witness Frame Ppre Qpre Rpre Qpre_temp Qpre_var)
+   (SETUP: call_setup2' cs Qtemp Qvar G a Delta P Q R argsig retty cc ts A Pre Post NEPre NEPost bl vl Qactuals
+      witness Frame Ppre Qpre Rpre Qpre_temp Qpre_var G')
    Espec
              (Post2: environ -> mpred)
              (B: Type)
@@ -3997,7 +4011,7 @@ Lemma semax_call_id01_wow:
 Proof.
 intros.
 destruct SETUP as [[PTREE [SPEC [ATY [TC0 [TC1 [MSUBST PTREE'']]]]]] 
-                            [PRE1 [PTREE' [CHECKTEMP [CHECKVAR FRAME]]]]].
+                            [PRE1 [PTREE' [CHECKTEMP [CHECKVAR [CHECKG FRAME]]]]]].
 apply SPEC. clear SPEC.
 eapply semax_pre_post';
    [ |
@@ -4026,7 +4040,7 @@ Qed.
 
 Ltac  forward_call_id1_wow' := 
 let H := fresh in intro H;
-eapply (semax_call_id1_wow _ _ _ _ _ _ _ _ _ _ _ _ _ _ _ _ _ _ _ _ _ _ _ _ _ _ _ H);
+eapply (semax_call_id1_wow _ _ _ _ _ _ _ _ _ _ _ _ _ _ _ _ _ _ _ _ _ _ _ _ _ _ _ _ H);
  clear H;
  lazymatch goal with Frame := _ : list mpred |- _ => try clear Frame end;
  [check_result_type
@@ -4044,7 +4058,7 @@ eapply (semax_call_id1_wow _ _ _ _ _ _ _ _ _ _ _ _ _ _ _ _ _ _ _ _ _ _ _ _ _ _ _
 
 Ltac forward_call_id1_x_wow' :=
 let H := fresh in intro H;
-eapply (semax_call_id1_x_wow _ _ _ _ _ _ _ _ _ _ _ _ _ _ _ _ _ _ _ _ _ _ _ _ _ _ _ H); 
+eapply (semax_call_id1_x_wow _ _ _ _ _ _ _ _ _ _ _ _ _ _ _ _ _ _ _ _ _ _ _ _ _ _ _ _ H); 
  clear H;
  lazymatch goal with Frame := _ : list mpred |- _ => try clear Frame end;
  [ check_result_type | check_result_type
@@ -4065,7 +4079,7 @@ eapply (semax_call_id1_x_wow _ _ _ _ _ _ _ _ _ _ _ _ _ _ _ _ _ _ _ _ _ _ _ _ _ _
 
 Ltac forward_call_id1_y_wow' :=
 let H := fresh in intro H;
-eapply (semax_call_id1_y_wow _ _ _ _ _ _ _ _ _ _ _ _ _ _ _ _ _ _ _ _ _ _ _ _ _ _ _ H); 
+eapply (semax_call_id1_y_wow _ _ _ _ _ _ _ _ _ _ _ _ _ _ _ _ _ _ _ _ _ _ _ _ _ _ _ _ H); 
  clear H;
  lazymatch goal with Frame := _ : list mpred |- _ => try clear Frame end;
  [ check_result_type | check_result_type
@@ -4085,7 +4099,7 @@ eapply (semax_call_id1_y_wow _ _ _ _ _ _ _ _ _ _ _ _ _ _ _ _ _ _ _ _ _ _ _ _ _ _
 
 Ltac forward_call_id01_wow' :=
 let H := fresh in intro H;
-eapply (semax_call_id01_wow _ _ _ _ _ _ _ _ _ _ _ _ _ _ _ _ _ _ _ _ _ _ _ _ _ _ _ H); 
+eapply (semax_call_id01_wow _ _ _ _ _ _ _ _ _ _ _ _ _ _ _ _ _ _ _ _ _ _ _ _ _ _ _ _ H); 
  clear H;
  lazymatch goal with Frame := _ : list mpred |- _ => try clear Frame end;
  [ apply Coq.Init.Logic.I 
@@ -4101,7 +4115,7 @@ eapply (semax_call_id01_wow _ _ _ _ _ _ _ _ _ _ _ _ _ _ _ _ _ _ _ _ _ _ _ _ _ _ 
 
 Ltac forward_call_id00_wow'  :=
 let H := fresh in intro H;
-eapply (semax_call_id00_wow _ _ _ _ _ _ _ _ _ _ _ _ _ _ _ _ _ _ _ _ _ _ _ _ _ _ _ H); 
+eapply (semax_call_id00_wow _ _ _ _ _ _ _ _ _ _ _ _ _ _ _ _ _ _ _ _ _ _ _ _ _ _ _ _ H); 
  clear H;
  lazymatch goal with Frame := _ : list mpred |- _ => try clear Frame end;
  [ check_result_type 
@@ -4124,7 +4138,7 @@ lazymatch goal with
       lazymatch goal with
       | |- _ -> semax _ _ (Scall (Some _) _ _) _ =>
          forward_call_id1_wow'
-      | |- call_setup2' _ _ _ _ _ _ _ _ _ ?retty _ _ _ _ _ _ _ _ _ _ _ _ _ _ _ _ _ -> 
+      | |- call_setup2' _ _ _ _ _ _ _ _ _ _ ?retty _ _ _ _ _ _ _ _ _ _ _ _ _ _ _ _ _ -> 
                 semax _ _ (Scall None _ _) _ =>
         tryif (unify retty Tvoid)
         then forward_call_id00_wow'
