floyd/client_lemmas.v
@@ -1470,6 +1470,11 @@ Proof.
       unfold local, lift1; unfold_lift; intros rho.
       unfold subst; simpl.
       apply derives_refl.
+    - rewrite !local_lift2_and.
+      apply andp_derives; [| exact IHQ].
+      unfold local, lift1; unfold_lift; intros rho.
+      unfold subst; simpl.
+      apply derives_refl.
 Qed.
 
 Fixpoint iota_formals (i: ident) (tl: typelist) :=
