floyd/local2ptree_denote.v
@@ -57,10 +57,11 @@ match Q with
       end
 (*| tc_env D => f T1 T2 P' (tc_env D :: Q') *)
 | localprop P => f T1 T2 (P :: P') Q'
+| gvars gv => f T1 T2 P' (gvars gv :: Q')
 end.
 
 Fixpoint local2ptree_aux (Q: list localdef)
-   (T1: PTree.t val) (T2: PTree.t vardesc) (P': list Prop) (Q': list localdef) :
+   (T1: PTree.t val) (T2: PTree.t vardesc) (P': list Prop) (Q': list localdef):
    local_trees :=
 match Q with
 | Q1 :: Qr => local2ptree1 Q1 T1 T2 P' Q' (local2ptree_aux Qr)
@@ -68,7 +69,7 @@ match Q with
 end.
 
 Definition local2ptree (Q: list localdef)
-     : (PTree.t val * PTree.t vardesc * list Prop * list localdef) :=
+     : (PTree.t val * PTree.t vardesc * list Prop * list localdef ) :=
 local2ptree_aux Q PTree.Leaf PTree.Leaf nil nil.
 
 Definition CLEAR_ME {T} (x:T) := x.
@@ -81,6 +82,7 @@ Ltac hnf_localdef_list A :=
  | gvar _ ?v :: ?Q' => hide_it v; hnf_localdef_list Q'
  | sgvar _ ?v :: ?Q' => hide_it v; hnf_localdef_list Q'
  | localprop ?v :: ?Q' => hide_it v; hnf_localdef_list Q'
+ | gvars ?v :: ?Q' => hide_it v; hnf_localdef_list Q'
 (* | tc_env ?v :: ?Q' => hide_it v;  hnf_localdef_list Q'      *)
   | ?B :: ?C => let x := eval hnf in B in change B with x; hnf_localdef_list (x::C)
   | nil => idtac
@@ -88,12 +90,23 @@ Ltac hnf_localdef_list A :=
             let x := eval hnf in A in (change A with x); hnf_localdef_list x
   end.
 
+Ltac grab_gvars L := 
+ match L with gvars ?A :: ?B => let x := grab_gvars B in let z := constr:(A::x) in z
+                | nil => let x := constr:(@nil globals) in x
+  end.
+
 Ltac prove_local2ptree :=
  clear;
  match goal with |- local2ptree ?A = _ => hnf_localdef_list A end;
- unfold local2ptree, local2ptree_aux; simpl;
- repeat match goal with x := CLEAR_ME _ |- _ => unfold CLEAR_ME in x; subst x end;
- reflexivity.
+ etransitivity;
+ [unfold local2ptree, local2ptree_aux; simpl;
+  repeat match goal with x := CLEAR_ME _ |- _ => unfold CLEAR_ME in x; subst x end;
+  reflexivity |
+  repeat match goal with x := CLEAR_ME _ |- _ => unfold CLEAR_ME in x; subst x end;
+  apply f_equal;
+  try reflexivity;
+  match goal with |- ?L = _ => let x := grab_gvars L in instantiate(1:=x); reflexivity end
+ ].
 
 Goal exists x,  local2ptree (
       temp 1%positive Vundef
@@ -1084,6 +1097,12 @@ Proof.
  +
     rewrite <- (IHQ _ _ _ _ _ _ _ _ H); clear IHQ H.
     simpl app. rewrite <- insert_prop. rewrite <- insert_local'. reflexivity.
+ +
+    rewrite <- (IHQ _ _ _ _ _ _ _ _ H); clear IHQ H.
+     apply LOCALx_shuffle'.
+     intros.
+     rewrite !in_app. rewrite LOCALx_expand_res.
+     rewrite !in_cns. clear; intuition.
 Qed.
 
 Lemma local2ptree_soundness  : forall P Q R T1 T2 P' Q',
