floyd/sc_set_load_store.v
@@ -585,8 +585,8 @@ Context {cs: compspecs}.
 
 Lemma semax_PTree_set:
   forall {Espec: OracleKind},
-    forall Delta id P Q R T1 T2 (e2: expr) t v,
-      local2ptree Q = (T1, T2, nil, nil) ->
+    forall Delta id P Q R T1 T2 G (e2: expr) t v,
+      local2ptree Q = (T1, T2, nil, G) ->
       typeof_temp Delta id = Some t ->
       is_neutral_cast (implicit_deref (typeof e2)) t = true ->
       msubst_eval_expr T1 T2 e2 = Some v ->
@@ -612,11 +612,11 @@ Qed.
 Lemma semax_PTree_field_load_no_hint:
   forall {Espec: OracleKind},
     forall n Rn Delta sh id P Q R (e: expr) t
-      T1 T2 e_root (efs: list efield) (tts: list type) lr
+      T1 T2 G e_root (efs: list efield) (tts: list type) lr
       t_root_from_e gfs_from_e p_from_e
       (t_root: type) (gfs0 gfs1 gfs: list gfield) (p: val)
       (v : val) (v' : reptype (nested_field_type t_root gfs0)),
-      local2ptree Q = (T1, T2, nil, nil) ->
+      local2ptree Q = (T1, T2, nil, G) ->
       compute_nested_efield e = (e_root, efs, tts, lr) ->
       typeof_temp Delta id = Some t ->
       is_neutral_cast (typeof e) t = true ->
@@ -641,7 +641,7 @@ Lemma semax_PTree_field_load_no_hint:
               (LOCALx (temp id v :: remove_localdef_temp id Q)
                 (SEPx R)))).
 Proof.
-  intros ? ? ? ? ? ? ? ? ? ? ?
+  intros ? ? ? ? ? ? ? ? ? ? ? ?
          ? ? ? ? ? ?
          ? ? ?
          ? ? ? ? ?
@@ -656,7 +656,7 @@ Proof.
   Focus 1. {
     erewrite (local2ptree_soundness P Q R) by eauto.
     simpl app.
-    apply (msubst_efield_denote_eq P _ _ nil R)  in EVAL_EFIELD.
+    apply (msubst_efield_denote_eq P _ _ G R)  in EVAL_EFIELD.
     eapply derives_trans; [apply andp_left2, EVAL_EFIELD |].
     intro rho; simpl; unfold local, lift1; unfold_lift.
     apply prop_derives; intros.
@@ -701,8 +701,8 @@ Proof.
     apply andp_left2.
     simpl app.
     apply andp_right.
-    + apply (msubst_efield_denote_eq P _ _ nil R) in EVAL_EFIELD; auto.
-    + apply (msubst_eval_LR_eq P _ _ nil R) in EVAL_ROOT; auto.
+    + apply (msubst_efield_denote_eq P _ _ G R) in EVAL_EFIELD; auto.
+    + apply (msubst_eval_LR_eq P _ _ G R) in EVAL_ROOT; auto.
   } Unfocus.
   eapply semax_SC_field_load.
   1: rewrite NESTED_EFIELD, <- TYPEOF, TYPE_EQ; reflexivity.
@@ -724,10 +724,10 @@ Qed.
 Lemma semax_PTree_field_load_with_hint:
   forall {Espec: OracleKind},
     forall n Rn Delta sh id P Q R (e: expr) t
-      T1 T2 p_from_e
+      T1 T2 G p_from_e
       (t_root: type) (gfs0 gfs1 gfs: list gfield) (p: val)
       (v_val : val) (v_reptype : reptype (nested_field_type t_root gfs0)),
-      local2ptree Q = (T1, T2, nil, nil) ->
+      local2ptree Q = (T1, T2, nil, G) ->
       typeof_temp Delta id = Some t ->
       is_neutral_cast (typeof e) t = true ->
       type_is_volatile (typeof e) = false ->
@@ -746,7 +746,7 @@ Lemma semax_PTree_field_load_with_hint:
             (LOCALx (temp id v_val :: remove_localdef_temp id Q)
               (SEPx R)))).
 Proof.
-  intros ? ? ? ? ? ? ? ? ? ?
+  intros ? ? ? ? ? ? ? ? ? ? ?
          ? ? ? ?
          ? ? ? ? ?
          ? ?
@@ -773,11 +773,11 @@ Qed.
 Lemma semax_PTree_field_cast_load_no_hint:
   forall {Espec: OracleKind},
     forall n Rn Delta sh id P Q R (e: expr) t
-      T1 T2 e_root (efs: list efield) (tts: list type) lr
+      T1 T2 G e_root (efs: list efield) (tts: list type) lr
       t_root_from_e gfs_from_e p_from_e
       (t_root: type) (gfs0 gfs1 gfs: list gfield) (p: val)
       (v : val) (v' : reptype (nested_field_type t_root gfs0)),
-      local2ptree Q = (T1, T2, nil, nil) ->
+      local2ptree Q = (T1, T2, nil, G) ->
       compute_nested_efield e = (e_root, efs, tts, lr) ->
       typeof_temp Delta id = Some t ->
       type_is_by_value (typeof e) = true ->
@@ -803,7 +803,7 @@ Lemma semax_PTree_field_cast_load_no_hint:
               (LOCALx (temp id (eval_cast (typeof e) t v) :: remove_localdef_temp id Q)
                 (SEPx R)))).
 Proof.
-  intros ? ? ? ? ? ? ? ? ? ? ?
+  intros ? ? ? ? ? ? ? ? ? ? ? ?
          ? ? ? ? ? ?
          ? ? ?
          ? ? ? ? ?
@@ -817,7 +817,7 @@ Proof.
   Focus 1. {
     erewrite (local2ptree_soundness P Q R) by eauto.
     simpl app.
-    apply (msubst_efield_denote_eq P _ _ nil R)  in EVAL_EFIELD.
+    apply (msubst_efield_denote_eq P _ _ G R)  in EVAL_EFIELD.
     eapply derives_trans; [apply andp_left2, EVAL_EFIELD |].
     intro rho; simpl; unfold local, lift1; unfold_lift.
     apply prop_derives; intros.
@@ -862,8 +862,8 @@ Proof.
     apply andp_left2.
     simpl app.
     apply andp_right.
-    + apply (msubst_efield_denote_eq P _ _ nil R) in EVAL_EFIELD; auto.
-    + apply (msubst_eval_LR_eq P _ _ nil R) in EVAL_ROOT; auto.
+    + apply (msubst_efield_denote_eq P _ _ G R) in EVAL_EFIELD; auto.
+    + apply (msubst_eval_LR_eq P _ _ G R) in EVAL_ROOT; auto.
   } Unfocus.
   rewrite NESTED_EFIELD. rewrite <- TYPEOF, TYPE_EQ.
   eapply semax_SC_field_cast_load.
@@ -887,10 +887,10 @@ Qed.
 Lemma semax_PTree_field_cast_load_with_hint:
   forall {Espec: OracleKind},
     forall n Rn Delta sh id P Q R (e: expr) t
-      T1 T2 p_from_e
+      T1 T2 G p_from_e
       (t_root: type) (gfs0 gfs1 gfs: list gfield) (p: val)
       (v_val : val) (v_reptype : reptype (nested_field_type t_root gfs0)),
-      local2ptree Q = (T1, T2, nil, nil) ->
+      local2ptree Q = (T1, T2, nil, G) ->
       typeof_temp Delta id = Some t ->
       type_is_by_value (typeof e) = true ->
       type_is_volatile (typeof e) = false ->
@@ -910,7 +910,7 @@ Lemma semax_PTree_field_cast_load_with_hint:
             (LOCALx (temp id (eval_cast (typeof e) t v_val) :: remove_localdef_temp id Q)
               (SEPx R)))).
 Proof.
-  intros ? ? ? ? ? ? ? ? ? ?
+  intros ? ? ? ? ? ? ? ? ? ? ?
          ? ? ? ?
          ? ? ? ? ?
          ? ?
@@ -939,12 +939,12 @@ Qed.
 Lemma semax_PTree_field_store_no_hint:
   forall {Espec: OracleKind},
     forall n Rn Delta sh P Q R (e1 e2 : expr)
-      T1 T2 e_root (efs: list efield) (tts: list type) lr
+      T1 T2 G e_root (efs: list efield) (tts: list type) lr
       t_root_from_e gfs_from_e p_from_e
       (t_root: type) (gfs0 gfs1 gfs: list gfield) (p: val) 
       (v0: reptype (nested_field_type (nested_field_type t_root gfs0) gfs1))
       (v0_val: val) Rv (v v_new: reptype (nested_field_type t_root gfs0)),
-      local2ptree Q = (T1, T2, nil, nil) ->
+      local2ptree Q = (T1, T2, nil, G) ->
       compute_nested_efield e1 = (e_root, efs, tts, lr) ->
       type_is_by_value (typeof e1) = true ->
       type_is_volatile (typeof e1) = false ->
@@ -971,7 +971,7 @@ Lemma semax_PTree_field_store_no_hint:
                 (SEPx
                   (replace_nth n R (Rv v_new)))))).
 Proof.
-  intros ? ? ? ? ? ? ? ? ? ?
+  intros ? ? ? ? ? ? ? ? ? ? ?
          ? ? ? ? ? ?
          ? ? ? ?
          ? ? ? ? ?
@@ -985,7 +985,7 @@ Proof.
   Focus 1. {
     erewrite (local2ptree_soundness P Q R) by eauto.
     simpl app.
-    apply (msubst_efield_denote_eq P _ _ nil R)  in EVAL_EFIELD.
+    apply (msubst_efield_denote_eq P _ _ G R)  in EVAL_EFIELD.
     eapply derives_trans; [apply andp_left2, EVAL_EFIELD |].
     intro rho; simpl; unfold local, lift1; unfold_lift.
     apply prop_derives; intros.
@@ -1030,8 +1030,8 @@ Proof.
     apply andp_left2.
     simpl app.
     apply andp_right.
-    + apply (msubst_efield_denote_eq P _ _ nil R) in EVAL_EFIELD; auto.
-    + apply (msubst_eval_LR_eq P _ _ nil R) in EVAL_ROOT; auto.
+    + apply (msubst_efield_denote_eq P _ _ G R) in EVAL_EFIELD; auto.
+    + apply (msubst_eval_LR_eq P _ _ G R) in EVAL_ROOT; auto.
   } Unfocus.
   rewrite NESTED_EFIELD.
   eapply semax_SC_field_store.
@@ -1057,11 +1057,11 @@ Qed.
 Lemma semax_PTree_field_store_with_hint:
   forall {Espec: OracleKind},
     forall n Rn Delta sh P Q R (e1 e2 : expr)
-      T1 T2 p_from_e
+      T1 T2 G p_from_e
       (t_root: type) (gfs0 gfs1 gfs: list gfield) (p: val) 
       (v0: reptype (nested_field_type (nested_field_type t_root gfs0) gfs1))
       (v0_val: val) Rv (v v_new: reptype (nested_field_type t_root gfs0)),
-      local2ptree Q = (T1, T2, nil, nil) ->
+      local2ptree Q = (T1, T2, nil, G) ->
       type_is_by_value (typeof e1) = true ->
       type_is_volatile (typeof e1) = false ->
       msubst_eval_expr T1 T2 (Ecast e2 (typeof e1)) = Some v0_val ->
@@ -1084,7 +1084,7 @@ Lemma semax_PTree_field_store_with_hint:
                   (replace_nth n R
                     (field_at sh t_root gfs0 v_new p)))))).
 Proof.
-  intros ? ? ? ? ? ? ? ? ? ?
+  intros ? ? ? ? ? ? ? ? ? ? ?
          ? ? ? ?
          ? ? ? ? ? ?
          ? ? ?
@@ -1280,16 +1280,18 @@ Ltac load_tac_no_hint LOCAL2PTREE :=
                                                          "unexpected failure in entailer_for_load_tac"]
   ].
 
+
 Ltac load_tac :=
   match goal with
   | |- semax ?Delta (|> (PROPx ?P (LOCALx ?Q (SEPx ?R)))) (Sset _ ?e) _ =>
     let T1 := fresh "T1" in evar (T1: PTree.t val);
     let T2 := fresh "T2" in evar (T2: PTree.t vardesc);
+    let G := fresh "G" in evar (G: list localdef);
     let LOCAL2PTREE := fresh "LOCAL2PTREE" in
-    assert (local2ptree Q = (T1, T2, nil, nil)) as LOCAL2PTREE;
-    [subst T1 T2; prove_local2ptree |];
+    assert (local2ptree Q = (T1, T2, nil, G)) as LOCAL2PTREE;
+    [subst T1 T2 G; prove_local2ptree |];
     first [ load_tac_with_hint LOCAL2PTREE | load_tac_no_hint LOCAL2PTREE | SEP_type_contradict LOCAL2PTREE e R | hint_msg LOCAL2PTREE e];
-    clear T1 T2 LOCAL2PTREE
+    clear T1 T2 G LOCAL2PTREE
   end.
 
 Ltac cast_load_tac_with_hint LOCAL2PTREE :=
@@ -1342,11 +1344,12 @@ Ltac cast_load_tac :=
   | |- semax ?Delta (|> (PROPx ?P (LOCALx ?Q (SEPx ?R)))) (Sset _ (Ecast ?e _)) _ =>
     let T1 := fresh "T1" in evar (T1: PTree.t val);
     let T2 := fresh "T2" in evar (T2: PTree.t vardesc);
+    let G := fresh "G" in evar (G: list localdef);
     let LOCAL2PTREE := fresh "LOCAL2PTREE" in
-    assert (local2ptree Q = (T1, T2, nil, nil)) as LOCAL2PTREE;
-    [subst T1 T2; prove_local2ptree |];
+    assert (local2ptree Q = (T1, T2, nil, G)) as LOCAL2PTREE;
+    [subst T1 T2 G; prove_local2ptree |];
     first [ cast_load_tac_with_hint LOCAL2PTREE | cast_load_tac_no_hint LOCAL2PTREE | SEP_type_contradict LOCAL2PTREE e R | hint_msg LOCAL2PTREE e];
-    clear T1 T2 LOCAL2PTREE
+    clear T1 T2 G LOCAL2PTREE
   end.
 
 Lemma data_equal_congr {cs: compspecs}:
@@ -1410,9 +1413,10 @@ Ltac store_tac :=
   | |- semax ?Delta (|> (PROPx ?P (LOCALx ?Q (SEPx ?R)))) (Sassign ?e1 ?e2) _ =>
     let T1 := fresh "T1" in evar (T1: PTree.t val);
     let T2 := fresh "T2" in evar (T2: PTree.t vardesc);
+    let G := fresh "G" in evar (G: list localdef);
     let LOCAL2PTREE := fresh "LOCAL2PTREE" in
-    assert (local2ptree Q = (T1, T2, nil, nil)) as LOCAL2PTREE;
-    [subst T1 T2; prove_local2ptree |];
+    assert (local2ptree Q = (T1, T2, nil, G)) as LOCAL2PTREE;
+    [subst T1 T2 G; prove_local2ptree |];
     first [ store_tac_with_hint LOCAL2PTREE | store_tac_no_hint LOCAL2PTREE | SEP_type_contradict LOCAL2PTREE e1 R | hint_msg LOCAL2PTREE e1];
     clear T1 T2 LOCAL2PTREE
   end.
