progs/verif_nest2.v
@@ -10,50 +10,61 @@ Definition t_struct_b := Tstruct _b noattr.
 
 Definition get_spec :=
  DECLARE _get
-  WITH v : reptype' t_struct_b, p : val
+  WITH v : reptype' t_struct_b, gv: globals
   PRE  []
         PROP ()
-        LOCAL(gvar _p p)
-        SEP(data_at Ews t_struct_b (repinj _ v) p)
+        LOCAL(gvars gv)
+        SEP(data_at Ews t_struct_b (repinj _ v) (gv _p))
   POST [ tint ]
          PROP()
          LOCAL (temp 1%positive (Vint (snd (snd v))))
-         SEP (data_at Ews t_struct_b (repinj _ v) p).
+         SEP (data_at Ews t_struct_b (repinj _ v) (gv _p)).
 
 Definition get_spec' :=
  DECLARE _get
-  WITH v : (int * (float * int))%type, p : val
+  WITH v : (int * (float * int))%type, gv: globals
   PRE  []
         PROP ()
-        LOCAL(gvar _p p)
-        SEP(data_at Ews t_struct_b (repinj t_struct_b v) p)
+        LOCAL(gvars gv)
+        SEP(data_at Ews t_struct_b (repinj t_struct_b v) (gv _p))
   POST [ tint ]
          PROP()
          LOCAL (temp 1%positive (Vint (snd (snd v))))
-         SEP (data_at Ews t_struct_b (repinj t_struct_b v) p).
+         SEP (data_at Ews t_struct_b (repinj t_struct_b v) (gv _p)).
 
 Definition update22 (i: int) (v: reptype' t_struct_b) : reptype' t_struct_b :=
    (fst v, (fst (snd v), i)).
 
 Definition set_spec :=
  DECLARE _set
-  WITH i : int, v : reptype' t_struct_b, p : val
+  WITH i : int, v : reptype' t_struct_b, gv: globals
   PRE  [ _i OF tint ]
          PROP  ()
-         LOCAL (gvar _p p;
+         LOCAL (gvars gv;
                 temp _i (Vint i))
-         SEP   (data_at Ews t_struct_b (repinj _ v) p)
+         SEP   (data_at Ews t_struct_b (repinj _ v) (gv _p))
   POST [ tvoid ]
          PROP() LOCAL()
-        SEP(data_at Ews t_struct_b (repinj _ (update22 i v)) p).
+        SEP(data_at Ews t_struct_b (repinj _ (update22 i v)) (gv _p)).
 
 Definition Gprog : funspecs :=   ltac:(with_library prog [get_spec; set_spec]).
+
+Lemma gvars_denote1_i:
+  forall gv i v rho, gvar_denote i v rho -> gvars_denote gv rho -> gv i = v.
+Proof.
+intros.
+hnf in H,H0.
+subst.
+destruct (Map.get (ve_of rho) i) as [ [? ?] |] ; try contradiction.
+destruct (ge_of rho i); try contradiction; auto.
+Qed.
 
 Lemma body_get:  semax_body Vprog Gprog f_get get_spec.
 Proof.
 start_function.
 simpl in v.
 unfold_repinj.
+assert_gvar _p.
 Time forward. (* 5.989 sec  -> 2.6 -> 1.5 *)
 Time forward. (* 11.1118 sec -> 7.5 *)
 Time Qed.
@@ -63,6 +74,7 @@ Proof.
 start_function.
 simpl in v.
 unfold_repinj.
+assert_gvar _p.
 Time forward. (* 5.989 sec  -> 2.6*)
 Time forward. (* 11.1118 sec -> 7.5 *)
 Qed.
@@ -73,6 +85,7 @@ Proof.
 simpl in v.
 (*destruct v as [a [b c]]; simpl in *. *)
 unfold_repinj.
+assert_gvar _p.
 Time forward. (* 1.23 sec *)
 Time forward. (* 8.77  -> 5.25 sec *)
 Time Qed.  (*  28 sec -> 3.45 sec *)
