sha/verif_hmac_simple.v
@@ -35,9 +35,9 @@ Time forward_if  (
   PROP  (isptr c)
    LOCAL  (lvar _c t_struct_hmac_ctx_st c; temp _md md; temp _key k;
    temp _key_len (Vint (Int.repr kl)); temp _d d;
-   temp _n (Vint (Int.repr dl)); gvar sha._K256 kv)
+   temp _n (Vint (Int.repr dl)); gvars gv)
    SEP  (data_at_ Tsh t_struct_hmac_ctx_st c; data_block Tsh key k;
-   data_block Tsh data d; K_vector kv;
+   data_block Tsh data d; K_vector gv;
    memory_block shmd 32 md)).
   (*3.3*)
   { clear H. apply denote_tc_test_eq_split.
@@ -50,7 +50,7 @@ freeze [2;4] FR1.
 assert_PROP (isptr k) as isPtrK.
 { unfold data_block. Time normalize. (*1.6 versus 2.2*) rewrite data_at_isptr with (p:=k). Time entailer!. (*1.6 versus 2.5*) }
 
-Time forward_call (c, k, kl, key, kv, HMACabs nil nil nil). (*3*)
+Time forward_call (c, k, kl, key, HMACabs nil nil nil, gv). (*3*)
  { apply isptrD in isPtrK. destruct isPtrK as [kb [kofs HK]]. rewrite HK.
    unfold initPre. Time entailer!. (*0.6 versus 1.1*)
  }
@@ -62,12 +62,12 @@ destruct H as [H0_len512 FC_c].
 thaw FR2.
 thaw FR1.
 freeze [0;3] FR3.
-Time forward_call (hmacInit key, c, d, dl, data, kv). (*2.8*)
+Time forward_call (hmacInit key, c, d, dl, data, gv). (*2.8*)
   { rewrite H0_len512; assumption. }
 
 thaw FR3.
 freeze [2;3] FR4.
-Time forward_call (hmacUpdate data (hmacInit key), c, md, shmd, kv). (*2.3*)
+Time forward_call (hmacUpdate data (hmacInit key), c, md, shmd, gv). (*2.3*)
 freeze [0;2;3] FR5.
 forward_call (fst (hmacFinal (hmacUpdate data (hmacInit key))), c).
 freeze [0;1] FR6.
