sha/verif_sha_bdo.v
@@ -25,7 +25,7 @@ forward. (* data = in; *)
  semax_frame [ lvar _X (tarray tuint 16) Xv  ]
              [data_at_ Tsh (tarray tuint 16) Xv;
                       data_block sh (intlist_to_Zlist b) data;
-                      K_vector kv].
+                      K_vector gv].
  simple apply sha256_block_load8 with (ctx:=ctx); assumption.
 }
 eapply semax_seq'. {
@@ -36,7 +36,7 @@ eapply semax_seq'. {
   match goal with |- semax ?D _ _ _ => 
      replace D with Delta_loop1 by  (unfold Delta_loop1; repeat f_equal)
   end.
-  simple apply (sha256_block_data_order_loop1_proof _ sh b ctx data regs kv Xv); auto.
+  simple apply (sha256_block_data_order_loop1_proof _ sh b ctx data regs gv Xv); auto.
 }
 eapply semax_seq'. {
   semax_frame  [ ]
@@ -52,7 +52,7 @@ eapply semax_seq'. {
 }
 eapply seq_assocN with (cs := add_them_back). {
   semax_frame  [  lvar _X (tarray tuint 16) Xv ]
-             [K_vector kv;
+             [K_vector gv;
              data_at_ Tsh (tarray tuint LBLOCKz) Xv;
              data_block sh (intlist_to_Zlist b) data].
   simpl update_tycon.
